Updates

intermediate2/Zeta.Intermediate.Thread.fst
@@ -1,6 +1,8 @@
 module Zeta.Intermediate.Thread
 
 open FStar.Classical
+open Zeta.BinTree
+open Zeta.Record
 open Zeta.Intermediate.VerifierConfig
 open Zeta.Intermediate.SlotKeyRel
 
@@ -501,6 +503,101 @@ let verifiable_implies_valid_log_entry
     assert(valid_logS_entry s2ks e);
 
     ()
+
+let sp_is_mp (#vcfg:_) (tl: verifiable_log vcfg)
+  = let st = store tl in
+    slot_points_to_is_merkle_points_to st
+
+let sp_is_mp_empty (#vcfg:_) (tl: verifiable_log vcfg)
+  : Lemma (ensures (length tl = 0 ==> sp_is_mp tl))
+  = ()
+
+#push-options "--fuel 1 --ifuel 1 --z3rlimit_factor 3 --query_stats"
+
+let sp_is_mp_snoc_addm (#vcfg:_) (tl: verifiable_log vcfg {length tl > 0})
+  : Lemma (requires (let i = length tl - 1 in
+                     let tl' = prefix tl i in
+                     let e = index tl i in
+                     sp_is_mp tl' /\
+                     GV.AddM? e))
+          (ensures (sp_is_mp tl))
+  = let i = length tl - 1 in
+    let vs1 = state tl in
+    let st1 = vs1.st in
+
+    let tl' = prefix tl i in
+    let vs = state tl' in
+    let st = vs.st in
+
+    let e = index tl i in
+    let GV.AddM r s s' = e in
+    let a = AMP s r s' vs in
+    lemma_state_transition tl i;
+    assert(vs1 == GV.verify_step e vs);
+
+    let aux (s1 s2 dx:_)
+      : Lemma (ensures (slot_points_to_is_merkle_points_to_local st1 s1 s2 dx))
+      = assert(slot_points_to_is_merkle_points_to_local st s1 s2 dx);
+        if points_to_dir st1 s1 dx s2 then (
+          if s1 = s then (
+            assume(False); (**)
+            assert(points_to_dir st s' (addm_dir a) s2);
+            assert(slot_points_to_is_merkle_points_to_local st (addm_anc_slot a) s2 (addm_dir a));
+            assert(s2 <> s);
+            assert(s2 <> s');
+            lemma_addm_identical_except2 vs e s2
+          )
+          else if s1 = s' then (
+            if s2 = s then (
+              let mv1' = to_merkle_value (stored_value st1 s') in
+              let d = addm_dir a in
+              assert(addm_anc_val_postcond a mv1');
+
+              if d = dx then admit() (**)
+              else (
+                assume(False);
+                // let mv' = to_merkle_value (stored_value st s') in
+                // assert(desc_hash_dir mv1' dx = desc_hash_dir mv' dx);
+                assert(addm_anc_slot_points_postcond a st1);
+                assert(points_to_info st1 s' dx = points_to_info st s' dx);
+                assert(points_to_dir st1 s' dx s2);
+                assert(points_to_dir st s' dx s2);
+                ()
+              )
+            )
+            else (
+              assert(s2 <> s);
+              if s2 = s' then (
+                assume(False);
+                assert(slot_points_to_is_merkle_points_to_local st s' s' dx);
+                ()
+              )
+              else (
+                assume(False); (**)
+                assert(get_slot st s2 = get_slot st1 s2);
+                assert(addm_anc_slot_points_postcond a st1);
+                assert(dx = other_dir (addm_dir a));
+                assert(s1 = addm_anc_slot a);
+                assert(points_to_info st1 s' dx = points_to_info st s' dx);
+                assert(points_to_dir st s' dx s2);
+                assert(stored_key st s' = stored_key st1 s');
+                ()
+              )
+            )
+          )
+          else (
+            lemma_addm_identical_except2 vs e s1;
+            assert(inuse_slot st s1);
+            assert(inuse_slot st1 s1);
+            assert(stored_value st1 s1 = stored_value st s1);
+            assume(points_to_info st1 s1 dx = points_to_info st s1 dx);
+            ()
+          )
+        )
+    in
+    forall_intro_3 aux
+
+#pop-options
 
 let lemma_slot_is_merkle_points_to (#vcfg:_) (tl: verifiable_log vcfg)
   : Lemma (ensures (let st = store tl in
